concurrency/verif_bst_conc_atomic_delete.v
@@ -1,0 +1,246 @@
+Require Import VST.progs.conclib.
+Require Import VST.floyd.proofauto.
+Require Import VST.floyd.library.
+Require Import bst.bst_conc.
+Require Import VST.atomics.general_locks.
+Require Import bst.verif_bst_conc_atomic.
+
+Definition SEP_index : list Z := upto 22.
+
+Lemma body_pushdown_left: semax_body Vprog Gprog f_pushdown_left pushdown_left_spec.
+Proof.
+  start_function.
+  forward_loop (
+    EX p : val, EX lockp: val, EX tb : val, EX lockb: val, EX gb : gname,
+    PROP ()
+    LOCAL (temp _tgp p;  gvars gv)
+    SEP (atomic_shift (λ BST : tree, !! sorted_tree BST && tree_rep2 g g_root BST) ∅ ⊤
+        (λ (BST : tree) (_ : ()), fold_right_sepcon [!! sorted_tree (delete x BST) && tree_rep2 g g_root (delete x BST)])
+        (λ _ : (), Q);
+        mem_mgr gv;
+        in_tree g g_root; my_half g_root (range, Some (x, vx, ga, gb));
+        field_at Ews t_struct_tree_t [StructField _t] tp p;
+        data_at Ews t_struct_tree (vint x, (vx, (ta, tb))) tp; 
+        ltree g g_root lsh2 p lockp;
+        ltree g ga lsh1 ta locka; ltree g gb lsh1 tb lockb;
+        malloc_token Ews t_struct_tree tp;
+        malloc_token Ews tlock lockp;
+        malloc_token Ews t_struct_tree_t p))%assert.
+  { Exists p lockp tb lockb gb. entailer!. }
+  Intros p' lockp' tb' lockb' gb'.
+  unfold ltree at 1; Intros.
+  forward.
+  forward.
+  forward.
+  unfold ltree at 2; Intros.
+  forward.
+  forward_call (lockb', lsh1, node_lock_inv g tb' gb' lockb').
+  Local Typeclasses eauto := 5.
+  Time setoid_rewrite node_lock_inv_def at 2.
+  Intros b; destruct b as (rangeb, g_infob).
+  rewrite node_rep_def. Intros tbv; simpl.
+  forward.
+  Time forward_if.
+  { freeze FR_ghostb := (in_tree _ gb') (tree_rep_R tbv _ _ _) (my_half gb' _).
+    freeze FR_lockb := (lock_inv lsh1 lockb' _) (lock_inv lsh2 lockb' _)
+      (field_at Ews _ [StructField _t] _ tb') (malloc_token _ _ tb')
+      (field_at lsh2 _ [StructField _lock] _ tb') (malloc_token _ _ lockb')
+      (field_at lsh1 _ [StructField _lock] _ tb').
+    freeze FR_p := (lock_inv lsh2 lockp' _) (malloc_token _ _ tp) (malloc_token _ _ lockp')
+      (malloc_token _ _ p') (field_at lsh2 _ [StructField _lock] _ p').
+    forward.
+    unfold ltree at 1; Intros.
+    forward.
+    Time forward_call (locka, lsh1, node_lock_inv g ta ga locka).
+    Time setoid_rewrite node_lock_inv_def at 2.
+    Intros a; destruct a as (rangea, g_infoa).
+    rewrite node_rep_def; Intros tav; simpl.
+    forward.
+    forward.
+    thaw FR_p.
+    forward_call (t_struct_tree, tp, gv).
+    { if_tac; entailer!. }
+    thaw FR_lockb.
+    freeze FR_p := (lock_inv lsh2 lockp' _) (malloc_token _ _ lockp')
+      (malloc_token _ _ p') (field_at lsh2 _ [StructField _lock] _ p') (field_at Ews _ [StructField _t] _ p').
+    freeze FR_a := (lock_inv lsh1 locka _) (field_at Ews t_struct_tree_t [StructField _t] _ ta)
+      (malloc_token _ _ ta) (in_tree _ ga) (tree_rep_R tav _ _ _) (my_half ga _)
+      (field_at lsh2 _ [StructField _lock] _ ta) (malloc_token _ _ locka) (lock_inv lsh2 locka _)
+      (field_at lsh1 _ [StructField _lock] _ ta).
+    forward_call (lockb', Ews, lsh2, node_lock_inv_pred g tb' gb' lockb', node_lock_inv g tb' gb' lockb').
+    { lock_props.
+      rewrite <- (lock_inv_share_join lsh1 lsh2 Ews lockb') by auto.
+      cancel. }
+    forward_call (tlock, lockb', gv).
+    { if_tac; entailer!. }
+    forward_call (t_struct_tree_t, tb', gv).
+    { if_tac.
+      { saturate_local. subst tb'. contradiction. }
+(*       { entailer!. } (* cannot do this because -> Anomaly "Uncaught exception Failure("hd")." *) *)
+      { unfold_data_at (data_at_ Ews t_struct_tree_t tb'). simpl; cancel.
+        erewrite <- (field_at_share_join _ _ Ews _ [StructField _lock] _ tb') by eauto.
+        cancel. }}
+    thaw FR_a.
+    forward.
+    forward_call (locka, Ews, lsh2, node_lock_inv_pred g ta ga locka, node_lock_inv g ta ga locka).
+    { lock_props.
+      rewrite <- (lock_inv_share_join lsh1 lsh2 Ews locka) by auto.
+      entailer!. }
+    forward.
+    forward_call (tlock, locka, gv).
+    { if_tac; entailer!. }
+    forward_call (t_struct_tree_t, ta, gv).
+    { if_tac.
+      { saturate_local. subst ta. contradiction. }
+      unfold_data_at (data_at_ Ews t_struct_tree_t ta).
+      cancel. simpl.
+      erewrite <- (field_at_share_join _ _ Ews _ [StructField _lock] _ ta) by eauto.
+      entailer!. }
+    thaw FR_p.
+    gather_SEP (atomic_shift _ _ _ _ _) (my_half g_root _) (in_tree g g_root).
+    viewshift_SEP 0 (Q * (my_half g_root (rangea, g_infoa) * in_tree g g_root)). {
+      go_lower. eapply sync_commit_gen1.
+      - intros. iIntros "[Ha Hb]". iDestruct "Hb" as "[% Hb]".
+        iPoseProof (extract_lemmas_for_treerep2 with "[Ha Hb]") as "Hadd".
+        + apply H5.
+        + iFrame.
+        + iDestruct "Hadd" as (n1 n2 o) "[Ha Hb]". iExists (n1, n2, o).
+          iModIntro. iFrame.
+      admit. }
+    forward_call (lockp', lsh2, node_lock_inv_pred g p' g_root lockp', node_lock_inv g p' g_root lockp').
+    { lock_props.
+      setoid_rewrite node_lock_inv_def at 2. Exists (rangea, g_infoa).
+      rewrite node_rep_def; simpl. Exists tav. cancel. }
+    unfold tree_rep_R. rewrite H3; simpl; Intros.
+    forward. admit. }
+  unfold tree_rep_R at 1. abbreviate_semax.
+  if_tac.
+  { Intros. contradiction. }
+  { Intros gbl gbr k v tbl tbr ltbl ltbr.
+    forward_call (p', tp, x, vx, ta, tb', tbv, k, v, tbl, tbr).
+(*     { admit. } (* Need fix in assert_PROP to handle later statements. *) *)
+    forward.
+    forward_call (lockp', lsh2, node_lock_inv_pred g p' g_root lockp', node_lock_inv g p' g_root lockp').
+    { lock_props.
+      setoid_rewrite node_lock_inv_def at 4.
+      Exists (range, Some (x, vx, ga, gb')).
+      rewrite node_rep_def; simpl. Exists tbv. cancel.
+      unfold tree_rep_R.
+      if_tac.
+      { contradiction. }
+      { Exists g_root gbr k v tb' tbr lockb' ltbr. cancel.
+        unfold ltree at 3. entailer!.
+        rewrite later_sepcon. cancel. }
+    Exists tb' lockb' tbl ltbl.
+    entailer!.
+    unfold ltree at 1.
+    entailer!. }
+Admitted.
+
+Definition delete_inv (b: val) (sh: share) (* (lock: val) *) (x: Z) (* (v: val) *) (g_root: gname) gv (inv_names : invG) (Q : mpred) (g:gname) : environ -> mpred :=
+  ( EX np: val, EX r: number * number * option ghost_info, EX g_in :gname, EX lock : val,
+  PROP ( check_key_exist x (fst r) = true )
+  LOCAL (temp _l lock; temp _tgt np; temp _t b; temp _x (vint x); (* temp _value v; *) gvars gv)
+  SEP (lock_inv sh lock (node_lock_inv g np g_in lock);
+  node_lock_inv g np g_in lock;
+(* lock_inv sh lock (sync_inv g_in (node_rep np g )); node_rep np g g_in r; my_half g_in r; *)
+  atomic_shift (λ BST : @tree val, tree_rep2 g g_root BST ) ∅ ⊤
+    (λ (BST : @tree val) (_ : ()),
+       fold_right_sepcon [tree_rep2 g g_root (delete x BST) ]) 
+    (λ _ : (), Q);
+    mem_mgr gv; data_at sh (tptr t_struct_tree_t) np b ;
+(*      !!(field_compatible t_struct_tree_t nil np) && *)
+    field_at sh t_struct_tree_t [StructField _lock] lock np))%assert.
+
+Set Default Timeout 30.
+
+Lemma body_delete: semax_body Vprog Gprog f_delete delete_spec.
+Proof.
+  start_function.
+  unfold nodebox_rep; Intros p.
+  unfold ltree; Intros.
+  forward.
+  forward.
+  forward_call (lockb, sh, node_lock_inv g p g_root lockb). (* acquire(_l); *)
+  setoid_rewrite node_lock_inv_def at 2.
+  Intros rp; destruct rp as (rangep, g_infop).
+  rewrite node_rep_def; Intros tpv; simpl.
+  forward_loop (delete_inv b sh (* lockb *) x g_root gv inv_names Q g).
+  { unfold delete_inv.
+    Exists (p) (rangep, g_infop) (g_root) (lockb).
+    go_lower. entailer!.
+    { admit. }
+    { setoid_rewrite node_lock_inv_def at 2.
+      Exists (rangep, g_infop). cancel.
+      rewrite node_rep_def. Exists tpv; simpl. cancel. }}
+  unfold delete_inv. clear dependent p. Intros p rp g_in lockp.
+  setoid_rewrite node_lock_inv_def at 2. Intros rp'; destruct rp' as (rangep', g_infop').
+  rewrite node_rep_def; Intros tpv'; simpl.
+  forward.
+  forward_if. (* p == NULL *)
+  { forward_call (lockp, lsh2, node_lock_inv_pred g p g_in lockp, node_lock_inv g p g_in lockp).
+    { lock_props.
+      setoid_rewrite node_lock_inv_def at 3. Exists (rangep', g_infop').
+      rewrite node_rep_def. Exists tpv'; simpl.
+      cancel. }
+    forward.
+    { admit. }}
+  { unfold tree_rep_R. if_tac.
+    { contradiction. }
+    { Intros gl gr k v pl pr lockl lockr.
+      forward. (* y = p->key *)
+      forward_if. (* x < y *)
+      { forward.
+        forward.
+        unfold ltree at 1; Intros.
+        forward.
+        forward_call (lockl, lsh1, node_lock_inv g pl gl lockl). (* acquire(_l); *)
+        forward_call (lockp, lsh2, node_lock_inv_pred g p g_in lockp, node_lock_inv g p g_in lockp).
+        { lock_props.
+          setoid_rewrite node_lock_inv_def at 5. Exists (rangep', g_infop').
+          rewrite node_rep_def. Exists tpv'; simpl.
+          unfold tree_rep_R.
+          if_tac.
+          { contradiction. }
+          { Exists (gl) (gr) k v pl pr lockl lockr. cancel.
+            unfold ltree at 1. entailer!.
+            rewrite later_sepcon.
+            cancel. }}
+        unfold delete_inv.
+        Exists (pl) (rangep', g_infop') (g_in) (lockl).
+        go_lower. entailer!.
+        { admit. }
+        admit.
+        (* rewrite t_lock_pred_def at 1. Intros t' tp'.
+        unfold t_lock_pred_base. Exists (t') (tp').
+        entailer!. *) }
+      forward_if. (* y < x *)
+      { admit. (* forward.
+        forward.
+        unfold ltree at 2; Intros.
+        forward.
+        forward_call (lockr, lsh1, t_lock_pred pr lockr). (* acquire(_l); *)
+        forward_call (lockp, lsh2, t_lock_pred_base p lockp, t_lock_pred p lockp).
+        { lock_props.
+          setoid_rewrite t_lock_pred_def at 4. Exists (tvp) (tp).
+          unfold node_rep. rewrite E.
+          Exists (pl) (pr) (lockl) (lockr). unfold ltree at 3.
+          entailer!.
+          rewrite later_sepcon.
+          cancel. }
+        unfold delete_inv.
+        Exists (pr) (lockr).
+        rewrite t_lock_pred_def at 1. Intros t' tp'.
+        unfold t_lock_pred_base. Exists t' tp'.
+        entailer!. *)
+        }
+      { (* else case *)
+        assert_PROP (field_compatible t_struct_tree_t [] p). {
+          entailer!.
+        }
+        forward_call (p, tp, lockp, k, v, lockl, lockr, pl, pr, gv).
+        { unfold ltree. entailer!. }
+        forward. }
+      }
+    }
+Qed.
